TransVal/ComputeProps.v
@@ -1,8 +1,156 @@
 Require Import List Arith.
 Require Import IL Annotation AutoIndTac Bisim Exp MoreExp Coherence Fresh Util.
 Require Import SetOperations Sim Var.
-Require Import sexp smt nofun noGoto Terminates bitvec Crash freeVars.
-Require Import tvalTactics TUtil Guards.
+Require Import bitvec sexp smt nofun noGoto freeVars.
+Require Import Compute tvalTactics TUtil GuardProps.
+
+Lemma term_ssa_eval_agree L L' s D s' (E:onv val) (E':onv val)
+ : ssa s D
+   -> noFun s
+   -> Terminates (L, E, s) (L', E', s')
+   -> agree_on eq (fst (getAnn D)) E E'.
+
+Proof.
+  intros.
+  general induction H1; invt ssa; try invt F.step;try invt noFun; simpl;
+  try reflexivity; isabsurd.
+  - exploit IHTerminates; [ | | reflexivity | reflexivity |]; eauto.
+   rewrite H7 in X; simpl in *. cset_tac; intuition.
+   hnf. hnf in X. intros.
+   unfold update in X. specialize (X x0).
+   assert (x0 ∈ D0 ++ {x; {}}) by (cset_tac; left; assumption).
+   specialize (X H10). decide (x === x0); eauto.
+    + rewrite  <- e0 in H8; exfalso; apply H4 ; assumption.
+  - exploit IHTerminates; [ | | reflexivity | reflexivity |]; eauto.
+    rewrite H9 in X; simpl in *. assumption.
+  - exploit IHTerminates; [| | reflexivity | reflexivity |]; eauto.
+    rewrite H10 in X; simpl in *; assumption.
+Qed.
+
+Lemma terminates_impl_star2:
+  forall L E s L' Es s',
+    noFun s
+    -> Terminates (L, E ,s ) (L', Es, s')
+    -> (star2 F.step (L, E, s) nil (L', Es, s'))
+       /\ ((exists e, s' = stmtReturn e) \/ (exists f X, s' = stmtGoto f X)).
+
+Proof.
+intros.
+general induction H0; eauto.
+-split; eauto; econstructor.
+- split; eauto; econstructor.
+- inversion H2; subst; try isabsurd.
+  + exploit (IHTerminates L' E' s'); try reflexivity.
+    * inversion H; subst; eauto.
+    * destruct X as [step X]; split.
+      { change (star2 F.step (L0, E0, stmtExp x e s) (filter_tau EvtTau nil) (L'0, Es, s'0)).
+        econstructor; eauto. destruct a; eauto; isabsurd. }
+      { destruct X; eauto. }
+  + exploit (IHTerminates L' E' s'); eauto.
+    * inversion H; subst; eauto.
+    * destruct X as [step X]; split.
+      { change (star2 F.step (L0, E0, stmtIf e s t)(filter_tau EvtTau nil) (L'0, Es, s'0)).
+        econstructor; eauto; destruct a; eauto; isabsurd. }
+      {destruct X; eauto. }
+Qed.
+
+Lemma terminates_impl_models :
+forall L s D E s' E',
+ssa  s D
+-> noFun s
+-> Terminates (L,E, s) (L, E', s')
+->  models (fun (f:pred) (x:vallst) => true)  E'  (translateStmt s source).
+
+Proof.
+intros.
+general induction H1; simpl.
+- assert (X: models (fun (_:pred) (_:vallst) => true) E0 (smtReturn e)).
+  + simpl. econstructor.
+  + case_eq (undef e); eauto; intros.
+    * simpl; split; eauto.
+      eapply (guard_true_if_eval); eauto.
+- case_eq (undefLift x); intros; simpl; eauto.
+  + split; eauto.
+       eapply (guardList_true_if_eval _ E0); eauto.
+- inv H; invt ssa; invt noFun; simpl in * |- *; subst.
+  + case_eq(undef e); intros; simpl; split; eauto.
+    * eapply (guard_true_if_eval _ E'0 e s v ); eauto.
+      eapply exp_eval_agree; eauto.
+      assert (A: agree_on eq (fst (getAnn (ann1 (D0, D') an))) E0 E'0).
+      { eapply (term_ssa_eval_agree L' L' (stmtExp x e s') _ s'0 _ _);
+        econstructor; eauto. }
+      { eapply (agree_on_incl  (bv:=Exp.freeVars e) (lv:=fst (getAnn (ann1 (D0, D') an)))); eauto. }
+    * split; eauto; subst.
+      assert (X1: exp_eval E'0 (Var x) = Some v).
+      { eapply (exp_eval_agree (E:= E0[x <- Some v])) ; eauto.
+        - simpl. eapply (agree_on_incl (bv:={x} ) (lv:= fst (getAnn an))); subst.
+          + eapply (term_ssa_eval_agree L' L' s' _ s'0 _ E'0); eauto.
+          + rewrite H11. unfold fst. cset_tac. right; rewrite H6; reflexivity.
+        - unfold exp_eval. unfold update. decide (x===x); eauto; isabsurd. }
+      assert (X2: exp_eval E'0 e = Some v).
+      { eapply exp_eval_agree; eauto.
+      assert (A: agree_on eq (fst (getAnn (ann1 (D0, D') an))) E0 E'0).
+        - eapply (term_ssa_eval_agree L' L' (stmtExp x e s') _ s'0 _ _);
+          econstructor; eauto.
+        - eapply (agree_on_incl  (bv:=Exp.freeVars e) (lv:=fst (getAnn (ann1 (D0, D') an)))); eauto. }
+      {  unfold evalSexp. rewrite X1; rewrite X2.
+         eapply  bvEq_equiv_eq. reflexivity. }
+    * assert (X1: exp_eval E'0 (Var x) = Some v).
+      { eapply (exp_eval_agree (E:= E0 [x <- Some v])) ; eauto.
+        - simpl. eapply (agree_on_incl (bv:={x} ) (lv:= fst (getAnn an))).
+          + eapply (term_ssa_eval_agree L' L' s' _ s'0 _ _); eauto.
+          + rewrite H11. unfold fst. cset_tac. right; rewrite H6; reflexivity.
+        - unfold exp_eval. unfold update. decide (x===x); eauto; isabsurd. }
+      assert (X2: exp_eval E'0 e = Some v).
+      { eapply exp_eval_agree; eauto.
+      assert (A: agree_on eq (fst (getAnn (ann1 (D0, D') an))) E0 E'0).
+        - eapply (term_ssa_eval_agree  L' L' (stmtExp x e s') _ s'0);
+          econstructor; eauto.
+        - eapply (agree_on_incl  (bv:=Exp.freeVars e) (lv:=fst (getAnn (ann1 (D0, D') an)))); eauto. }
+      {  unfold evalSexp. rewrite X1; rewrite X2.
+         eapply  bvEq_equiv_eq. reflexivity.  }
+ + assert (X: models  (fun (_:pred) (_:vallst) => true) E'0 ( ite e (translateStmt s' source) (translateStmt b2 source))).
+    * simpl. unfold evalSexp.
+      assert (Exp.freeVars e ⊆ fst (getAnn (ann2 (D0, D') ans ant)))
+        by (hnf; intros; hnf in H7; specialize (H7 a); exact (H7 H4)).
+      assert (agree_on eq (fst (getAnn (ann2 (D0, D') ans ant))) E' E'0)
+        by ( eapply (term_ssa_eval_agree L' L' (stmtIf e s' b2) _ s'0 _ _); econstructor; eauto).
+      erewrite (exp_eval_agree (E:=E') (E':=E'0)); eauto. simpl. rewrite condTrue.
+      eapply IHTerminates; eauto.
+      eapply (agree_on_incl (bv:= Exp.freeVars e) (lv:= fst (getAnn (ann2 (D0, D') ans ant)))); eauto.
+    * case_eq (undef e); intros; eauto.
+      { simpl; split; eauto.
+        - eapply (guard_true_if_eval  (fun (_:pred) (_:vallst) => true) E'0 e _ v); eauto.
+          assert (Exp.freeVars e ⊆ fst (getAnn (ann2 (D0, D') ans ant)))
+            by (hnf; intros; hnf in H7; specialize (H7 a); hnf; cset_tac; simpl;  exact (H7 H5)).
+          assert (agree_on eq (fst (getAnn (ann2 (D0, D') ans ant))) E' E'0)
+            by ( eapply (term_ssa_eval_agree L' L' (stmtIf e s' b2) _ s'0 _ _); econstructor; eauto).
+          eapply (exp_eval_agree (E:=E') (E':=E'0)); eauto.
+          eapply (agree_on_incl (bv:= Exp.freeVars e) (lv:= fst (getAnn (ann2 (D0, D') ans ant)))); eauto.
+      }
+ + assert (X: models  (fun (_:pred) (_:vallst) => true) E'0( ite e (translateStmt b1 source) (translateStmt s' source))).
+    * simpl. unfold evalSexp.
+      assert (Exp.freeVars e ⊆ fst (getAnn (ann2 (D0, D') ans ant)))
+        by (hnf; intros; hnf in H7; specialize (H7 a); exact (H7 H4)).
+      assert (agree_on eq (fst (getAnn (ann2 (D0, D') ans ant))) E' E'0)
+      by ( eapply (term_ssa_eval_agree L' L' (stmtIf e b1 s') _ s'0 _ _);econstructor;  eauto).
+      erewrite (exp_eval_agree (E:=E') (E':=E'0)); eauto. simpl. rewrite condFalse.
+      eapply IHTerminates; eauto.
+      eapply (agree_on_incl (bv:= Exp.freeVars e) (lv:= fst (getAnn (ann2 (D0, D') ans ant)))); eauto.
+    * case_eq (undef e); intros; eauto.
+      { simpl; split; eauto.
+        - eapply (guard_true_if_eval  (fun (_:pred) (_:vallst) => true) E'0 e _ v); eauto.
+          + assert (Exp.freeVars e ⊆ fst (getAnn (ann2 (D0, D') ans ant)))
+              by (hnf; intros; hnf in H7; specialize (H7 a); hnf; cset_tac; simpl;  exact (H7 H5)).
+            assert (agree_on eq (fst (getAnn (ann2 (D0, D') ans ant))) E' E'0)
+              by ( eapply (term_ssa_eval_agree L' L' (stmtIf e b1 s') _ s'0 _ _); econstructor; eauto).
+            eapply (exp_eval_agree (E:=E') (E':=E'0)); eauto.
+            eapply (agree_on_incl (bv:= Exp.freeVars e) (lv:= fst (getAnn (ann2 (D0, D') ans ant)))); eauto.
+      }
+ + specialize (H0 l Y); isabsurd.
+Qed.
+
+(** Lemmata for Crash **)
 
 Definition failed (σ:F.state)  := result (σ ) = None.
 
@@ -29,6 +177,7 @@ Proof.
     rewrite H10 in X; eauto.
 Qed.
 
+(** TODO MOVE **)
 Lemma undef_models:
 forall F E e g,
 (forall x, x ∈ Exp.freeVars e -> exists v, E x = Some v)
