TransVal/nofun.v
@@ -1,4 +1,4 @@
-Require Import IL Terminates Crash.
+Require Import IL Compute.
 
 Inductive noFun : stmt->Prop :=
 |noFunLet x e s :
